::: tip
这是一个提示
:::

![](/logo.png)

Euler's identity $e^{i\pi}+1=0$ is a beautiful formula in $\mathbb{R}^2$.

.$$\frac {\partial^r} {\partial \omega^r} \left(\frac {y^{\omega}} {\omega}\right)
= \left(\frac {y^{\omega}} {\omega}\right) \left\{(\log y)^r + \sum_{i=1}^r \frac {(-1)^i r \cdots (r-i+1) (\log y)^{r-i}} {\omega^i} \right\}$$.

# 测试

.$$\frac {\partial^r} {\partial \omega^r} \left(\frac {y^{\omega}} {\omega}\right)
= \left(\frac {y^{\omega}} {\omega}\right) \left\{(\log y)^r + \sum_{i=1}^r \frac {(-1)^i r \cdots (r-i+1) (\log y)^{r-i}} {\omega^i} \right\}$$..$$\frac {\partial^r} {\partial \omega^r} \left(\frac {y^{\omega}} {\omega}\right)
= \left(\frac {y^{\omega}} {\omega}\right) \left\{(\log y)^r + \sum_{i=1}^r \frac {(-1)^i r \cdots (r-i+1) (\log y)^{r-i}} {\omega^i} \right\}$$.

## 2

.$$\frac {\partial^r} {\partial \omega^r} \left(\frac {y^{\omega}} {\omega}\right)
= \left(\frac {y^{\omega}} {\omega}\right) \left\{(\log y)^r + \sum_{i=1}^r \frac {(-1)^i r \cdots (r-i+1) (\log y)^{r-i}} {\omega^i} \right\}$$..$$\frac {\partial^r} {\partial \omega^r} \left(\frac {y^{\omega}} {\omega}\right)
= \left(\frac {y^{\omega}} {\omega}\right) \left\{(\log y)^r + \sum_{i=1}^r \frac {(-1)^i r \cdots (r-i+1) (\log y)^{r-i}} {\omega^i} \right\}$$..$$\frac {\partial^r} {\partial \omega^r} \left(\frac {y^{\omega}} {\omega}\right)
= \left(\frac {y^{\omega}} {\omega}\right) \left\{(\log y)^r + \sum_{i=1}^r \frac {(-1)^i r \cdots (r-i+1) (\log y)^{r-i}} {\omega^i} \right\}$$..$$\frac {\partial^r} {\partial \omega^r} \left(\frac {y^{\omega}} {\omega}\right)
= \left(\frac {y^{\omega}} {\omega}\right) \left\{(\log y)^r + \sum_{i=1}^r \frac {(-1)^i r \cdots (r-i+1) (\log y)^{r-i}} {\omega^i} \right\}$$.

### 2-1

.$$\frac {\partial^r} {\partial \omega^r} \left(\frac {y^{\omega}} {\omega}\right)
= \left(\frac {y^{\omega}} {\omega}\right) \left\{(\log y)^r + \sum_{i=1}^r \frac {(-1)^i r \cdots (r-i+1) (\log y)^{r-i}} {\omega^i} \right\}$$..$$\frac {\partial^r} {\partial \omega^r} \left(\frac {y^{\omega}} {\omega}\right)
= \left(\frac {y^{\omega}} {\omega}\right) \left\{(\log y)^r + \sum_{i=1}^r \frac {(-1)^i r \cdots (r-i+1) (\log y)^{r-i}} {\omega^i} \right\}$$..$$\frac {\partial^r} {\partial \omega^r} \left(\frac {y^{\omega}} {\omega}\right)
= \left(\frac {y^{\omega}} {\omega}\right) \left\{(\log y)^r + \sum_{i=1}^r \frac {(-1)^i r \cdots (r-i+1) (\log y)^{r-i}} {\omega^i} \right\}$$..$$\frac {\partial^r} {\partial \omega^r} \left(\frac {y^{\omega}} {\omega}\right)
= \left(\frac {y^{\omega}} {\omega}\right) \left\{(\log y)^r + \sum_{i=1}^r \frac {(-1)^i r \cdots (r-i+1) (\log y)^{r-i}} {\omega^i} \right\}$$.

### 2-2

.$$\frac {\partial^r} {\partial \omega^r} \left(\frac {y^{\omega}} {\omega}\right)
= \left(\frac {y^{\omega}} {\omega}\right) \left\{(\log y)^r + \sum_{i=1}^r \frac {(-1)^i r \cdots (r-i+1) (\log y)^{r-i}} {\omega^i} \right\}$$..$$\frac {\partial^r} {\partial \omega^r} \left(\frac {y^{\omega}} {\omega}\right)
= \left(\frac {y^{\omega}} {\omega}\right) \left\{(\log y)^r + \sum_{i=1}^r \frac {(-1)^i r \cdots (r-i+1) (\log y)^{r-i}} {\omega^i} \right\}$$..$$\frac {\partial^r} {\partial \omega^r} \left(\frac {y^{\omega}} {\omega}\right)
= \left(\frac {y^{\omega}} {\omega}\right) \left\{(\log y)^r + \sum_{i=1}^r \frac {(-1)^i r \cdots (r-i+1) (\log y)^{r-i}} {\omega^i} \right\}$$..$$\frac {\partial^r} {\partial \omega^r} \left(\frac {y^{\omega}} {\omega}\right)
= \left(\frac {y^{\omega}} {\omega}\right) \left\{(\log y)^r + \sum_{i=1}^r \frac {(-1)^i r \cdots (r-i+1) (\log y)^{r-i}} {\omega^i} \right\}$$.

## 3

.$$\frac {\partial^r} {\partial \omega^r} \left(\frac {y^{\omega}} {\omega}\right)
= \left(\frac {y^{\omega}} {\omega}\right) \left\{(\log y)^r + \sum_{i=1}^r \frac {(-1)^i r \cdots (r-i+1) (\log y)^{r-i}} {\omega^i} \right\}$$..$$\frac {\partial^r} {\partial \omega^r} \left(\frac {y^{\omega}} {\omega}\right)
= \left(\frac {y^{\omega}} {\omega}\right) \left\{(\log y)^r + \sum_{i=1}^r \frac {(-1)^i r \cdots (r-i+1) (\log y)^{r-i}} {\omega^i} \right\}$$..$$\frac {\partial^r} {\partial \omega^r} \left(\frac {y^{\omega}} {\omega}\right)
= \left(\frac {y^{\omega}} {\omega}\right) \left\{(\log y)^r + \sum_{i=1}^r \frac {(-1)^i r \cdots (r-i+1) (\log y)^{r-i}} {\omega^i} \right\}$$..$$\frac {\partial^r} {\partial \omega^r} \left(\frac {y^{\omega}} {\omega}\right)
= \left(\frac {y^{\omega}} {\omega}\right) \left\{(\log y)^r + \sum_{i=1}^r \frac {(-1)^i r \cdots (r-i+1) (\log y)^{r-i}} {\omega^i} \right\}$$.

### 3-1

.$$\frac {\partial^r} {\partial \omega^r} \left(\frac {y^{\omega}} {\omega}\right)
= \left(\frac {y^{\omega}} {\omega}\right) \left\{(\log y)^r + \sum_{i=1}^r \frac {(-1)^i r \cdots (r-i+1) (\log y)^{r-i}} {\omega^i} \right\}$$..$$\frac {\partial^r} {\partial \omega^r} \left(\frac {y^{\omega}} {\omega}\right)
= \left(\frac {y^{\omega}} {\omega}\right) \left\{(\log y)^r + \sum_{i=1}^r \frac {(-1)^i r \cdots (r-i+1) (\log y)^{r-i}} {\omega^i} \right\}$$..$$\frac {\partial^r} {\partial \omega^r} \left(\frac {y^{\omega}} {\omega}\right)
= \left(\frac {y^{\omega}} {\omega}\right) \left\{(\log y)^r + \sum_{i=1}^r \frac {(-1)^i r \cdots (r-i+1) (\log y)^{r-i}} {\omega^i} \right\}$$..$$\frac {\partial^r} {\partial \omega^r} \left(\frac {y^{\omega}} {\omega}\right)
= \left(\frac {y^{\omega}} {\omega}\right) \left\{(\log y)^r + \sum_{i=1}^r \frac {(-1)^i r \cdots (r-i+1) (\log y)^{r-i}} {\omega^i} \right\}$$.

### 3-2
